theories/SubstI3.v
@@ -1,0 +1,148 @@
+Require Import Coq.Lists.List.
+Require Import ExtLib.Data.HList.
+Require Import MirrorCore.TypesI.
+Require Import MirrorCore.ExprI.
+Require Import MirrorCore.EnvI.
+
+Set Implicit Arguments.
+Set Strict Implicit.
+
+Fixpoint hlist_build {T U} (F : T -> Type) (f : forall x : T, U -> option (F x))
+           (ls : list T) (ls' : list U)
+: option (hlist F ls) :=
+  match ls as ls , ls' return option (hlist F ls) with
+    | nil , nil => Some Hnil
+    | l :: ls , l' :: ls' =>
+      match hlist_build F f ls ls' with
+        | None => None
+        | Some res =>
+          match f l l' with
+            | None => None
+            | Some x =>
+              Some (Hcons x res)
+          end
+      end
+    | _ , _ => None
+  end.
+
+Section subst.
+  Variable T : Type.
+  (** the [expr] type requires a notion of unification variable **)
+  Variable typ : Type.
+  Variable typD : list Type -> typ -> Type.
+  Variable expr : Type.
+  Variable Expr_expr : Expr typD expr.
+
+  Let uvar : Type := nat.
+
+  Class Subst :=
+  { lookup : uvar -> T -> option expr
+  ; domain : T -> list uvar
+  }.
+
+  Class SubstUpdate :=
+  { set : uvar -> expr -> T -> option T (** TODO: Should this be typed? **)
+  ; pull : uvar -> nat -> T -> option T
+  ; empty : T
+  }.
+
+  Class SubstOk (S : Subst) : Type :=
+  { WellFormed_subst : T -> Prop
+  ; substD : forall (tus tvs : tenv typ), T -> ResType typD tus tvs Prop
+  ; substD_lookup
+    : forall s uv e,
+        WellFormed_subst s ->
+        lookup uv s = Some e ->
+        forall tus tvs sD,
+          substD tus tvs s = Some sD ->
+          exists t val,
+            exists pf : Some t = nth_error tus uv,
+            exprD' tus tvs e t = Some val /\
+            forall us vs,
+              sD us vs ->
+              hlist_nth us uv = match pf in _ = t
+                                      return match t with
+                                               | Some x => typD nil x
+                                               | None => unit
+                                             end
+                                with
+                                  | eq_refl => val us vs
+                                end
+  ; WellFormed_domain : forall s ls,
+      WellFormed_subst s ->
+      domain s = ls ->
+      (forall n, In n ls <-> lookup n s <> None)
+  }.
+
+
+  Class SubstUpdateOk (S : Subst) (SU : SubstUpdate) (SOk : SubstOk S) :=
+  { WellFormed_empty : WellFormed_subst empty
+  ; substD_empty : forall tus tvs,
+                   exists P,
+                     substD tus tvs empty = Some P /\
+                     forall us vs, P us vs
+  ; set_sound
+    : forall uv e s s',
+        set uv e s = Some s' ->
+        WellFormed_subst s ->
+        WellFormed_subst s' /\
+        (forall tus tvs t val sD,
+           substD tus tvs s = Some sD ->
+           forall pf : Some t = nth_error tus uv,
+           exprD' tus tvs e t = Some val ->
+           exists sD', substD tus tvs s' = Some sD' /\
+           forall us vs,
+             sD' us vs ->
+             sD us vs /\
+             hlist_nth us uv = match pf in _ = t
+                                     return match t with
+                                              | Some x => typD nil x
+                                              | None => unit
+                                            end
+                               with
+                                 | eq_refl => val us vs
+                               end)
+  ; pull_sound
+    : forall s s' u n,
+        pull u n s = Some s' ->
+        WellFormed_subst s ->
+        WellFormed_subst s' /\
+        forall tus tus' tvs sD,
+          u = length tus ->
+          n = length tus' ->
+          substD (tus ++ tus') tvs s = Some sD ->
+          exists sD',
+            substD tus tvs s' = Some sD' /\
+            exists eus' : list expr,
+              exists us' : hlist (fun t => hlist (typD nil) tus -> hlist (typD nil) tvs -> typD nil t) tus',
+                @hlist_build _ _ _ (fun t e => exprD' tus tvs e t) tus' eus' = Some us' /\
+                forall us vs,
+                  let us' := hlist_map (fun t (x : hlist (typD nil) tus -> hlist (typD nil) tvs -> typD nil t) => x us vs) us' in
+                  sD' us vs ->
+                  sD (hlist_app us us') vs
+  }.
+
+  Variable Subst_subst : Subst.
+  Variable SubstOk_subst : SubstOk Subst_subst.
+
+  Definition Subst_Extends (a b : T) : Prop :=
+    forall tus tvs P Q,
+      substD tus tvs b = Some P ->
+      substD tus tvs a = Some Q ->
+      forall us vs, P us vs -> Q us vs.
+
+  (** TODO:
+   ** Should [mentionsU] be part of [Expr]?
+   **)
+  Variable mentionsU : uvar -> expr -> bool.
+
+  Class NormalizedSubstOk : Type :=
+  { lookup_normalized : forall s e u,
+      WellFormed_subst s ->
+      lookup u s = Some e ->
+      forall u' e',
+        lookup u' s = Some e' ->
+        mentionsU u' e = false
+  }.
+
+End subst.
